\begin{dmath*}
R = \frac{1}{{{\beta}}}
\end{dmath*}
\begin{dmath*}
KY = \frac{{{\rho}}}{\frac{1}{{{\beta}}}-\left(1-{{\delta}}\right)}
\end{dmath*}
\begin{dmath*}
CY = 1-{{\delta}}\, \frac{{{\rho}}}{\frac{1}{{{\beta}}}-\left(1-{{\delta}}\right)}
\end{dmath*}
% Equation 1
\begin{dmath}
{{y}}_{t}={{c}}_{t}\, \left(1-{{\delta}}\, \frac{{{\rho}}}{\frac{1}{{{\beta}}}-\left(1-{{\delta}}\right)}\right)+{{v}}_{t}\, {{\delta}}\, \frac{{{\rho}}}{\frac{1}{{{\beta}}}-\left(1-{{\delta}}\right)}
\end{dmath}
% Equation 2
\begin{dmath}
\frac{1}{{{\eta}}}\, {{r}}_{t+1}={{c}}_{t+1}-{{c}}_{t}
\end{dmath}
% Equation 3
\begin{dmath}
{{c}}_{t}\, {{\eta}}={{y}}_{t}-{{n}}_{t}
\end{dmath}
% Equation 4
\begin{dmath}
{{r}}_{t}=\left({{y}}_{t}-{{k}}_{t-1}\right)\, {{\rho}}\, \frac{1}{\frac{{{\rho}}}{\frac{1}{{{\beta}}}-\left(1-{{\delta}}\right)}}
\end{dmath}
% Equation 5
\begin{dmath}
{{k}}_{t}=\left(1-{{\delta}}\right)\, {{k}}_{t-1}+{{\delta}}\, {{v}}_{t}
\end{dmath}
% Equation 6
\begin{dmath}
{{y}}_{t}={{z}}_{t}+{{\rho}}\, {{k}}_{t-1}+{{n}}_{t}\, \left(1-{{\rho}}\right)
\end{dmath}
% Equation 7
\begin{dmath}
{{z}}_{t}={{\psi}}\, {{z}}_{t-1}+{{\epsilon_z}}_{t}
\end{dmath}
