\begin{dmath*}
R = \frac{1}{{{\beta}}}
\end{dmath*}
\begin{dmath*}
KY = \frac{{{\rho}}}{\frac{1}{{{\beta}}}-\left(1-{{\delta}}\right)}
\end{dmath*}
\begin{dmath*}
CY = 1-{{\delta}}\, \frac{{{\rho}}}{\frac{1}{{{\beta}}}-\left(1-{{\delta}}\right)}
\end{dmath*}
% Equation 1
\begin{dmath}
{{y}}=\left(1-{{\delta}}\, \frac{{{\rho}}}{\frac{1}{{{\beta}}}-\left(1-{{\delta}}\right)}\right)\, {{c}}+{{\delta}}\, \frac{{{\rho}}}{\frac{1}{{{\beta}}}-\left(1-{{\delta}}\right)}\, {{v}}
\end{dmath}
% Equation 2
\begin{dmath}
\frac{1}{{{\eta}}}\, {{r}}=0
\end{dmath}
% Equation 3
\begin{dmath}
{{c}}\, {{\eta}}={{y}}-{{n}}
\end{dmath}
% Equation 4
\begin{dmath}
{{r}}=\left({{y}}-{{k}}\right)\, {{\rho}}\, \frac{1}{\frac{{{\rho}}}{\frac{1}{{{\beta}}}-\left(1-{{\delta}}\right)}}
\end{dmath}
% Equation 5
\begin{dmath}
{{k}}=\left(1-{{\delta}}\right)\, {{k}}+{{\delta}}\, {{v}}
\end{dmath}
% Equation 6
\begin{dmath}
{{y}}={{z}}+{{\rho}}\, {{k}}+{{n}}\, \left(1-{{\rho}}\right)
\end{dmath}
% Equation 7
\begin{dmath}
{{z}}={{z}}\, {{\psi}}+{{\epsilon_z}}
\end{dmath}
