\begin{dmath*}
uc = {{\gamma}}\, {{C}}^{\left(-1\right)}
\end{dmath*}
\begin{dmath*}
ucp = {{\gamma}}\, {{C}}^{\left(-1\right)}
\end{dmath*}
\begin{dmath*}
ul = \left(-{{\psi}}\right)\, \left(1-{{L}}\right)^{\left(-1\right)}
\end{dmath*}
\begin{dmath*}
fk = \frac{{{\alpha}}\, {{Y}}}{{{K}}}
\end{dmath*}
\begin{dmath*}
fl = \frac{{{Y}}\, \left(1-{{\alpha}}\right)}{{{L}}}
\end{dmath*}
% Equation 1
\begin{dmath}
{uc}={{\beta}}\, {ucp}\, \left(1-{{\delta}}+{{R}}\right)
\end{dmath}
% Equation 2
\begin{dmath}
{{W}}=\frac{\left(-{ul}\right)}{{uc}}
\end{dmath}
% Equation 3
\begin{dmath}
{{K}}={{K}}\, \left(1-{{\delta}}\right)+{{I}}
\end{dmath}
% Equation 4
\begin{dmath}
{{Y}}={{C}}+{{I}}
\end{dmath}
% Equation 5
\begin{dmath}
{{Y}}={{A}}\, {{K}}^{{{\alpha}}}\, {{L}}^{1-{{\alpha}}}
\end{dmath}
% Equation 6
\begin{dmath}
{{MC}}=1
\end{dmath}
% Equation 7
\begin{dmath}
{{W}}={{MC}}\, {fl}
\end{dmath}
% Equation 8
\begin{dmath}
{{R}}={{MC}}\, {fk}
\end{dmath}
% Equation 9
\begin{dmath}
log\left({{A}}\right)=log\left({{A}}\right)\, {{\rho^A}}+{{\varepsilon^A}}
\end{dmath}
