\begin{dmath*}
uc = {{\gamma}}\, {{C}_{t}}^{\left(-1\right)}
\end{dmath*}
\begin{dmath*}
ucp = {{\gamma}}\, {{C}_{t+1}}^{\left(-1\right)}
\end{dmath*}
\begin{dmath*}
ul = \left(-{{\psi}}\right)\, \left(1-{{L}_{t}}\right)^{\left(-1\right)}
\end{dmath*}
\begin{dmath*}
fk = \frac{{{\alpha}}\, {{Y}_{t}}}{{{K}_{t-1}}}
\end{dmath*}
\begin{dmath*}
fl = \frac{{{Y}_{t}}\, \left(1-{{\alpha}}\right)}{{{L}_{t}}}
\end{dmath*}
% Equation 1
\begin{dmath}
{uc_{t}}={{\beta}}\, {ucp_{t}}\, \left(1-{{\delta}}+{{R}_{t}}\right)
\end{dmath}
% Equation 2
\begin{dmath}
{{W}_{t}}=\frac{\left(-{ul_{t}}\right)}{{uc_{t}}}
\end{dmath}
% Equation 3
\begin{dmath}
{{K}_{t}}={{K}_{t-1}}\, \left(1-{{\delta}}\right)+{{I}_{t}}
\end{dmath}
% Equation 4
\begin{dmath}
{{Y}_{t}}={{C}_{t}}+{{I}_{t}}
\end{dmath}
% Equation 5
\begin{dmath}
{{Y}_{t}}={{A}_{t}}\, {{K}_{t-1}}^{{{\alpha}}}\, {{L}_{t}}^{1-{{\alpha}}}
\end{dmath}
% Equation 6
\begin{dmath}
{{MC}_{t}}=1
\end{dmath}
% Equation 7
\begin{dmath}
{{W}_{t}}={{MC}_{t}}\, {fl_{t}}
\end{dmath}
% Equation 8
\begin{dmath}
{{R}_{t}}={{MC}_{t}}\, {fk_{t}}
\end{dmath}
% Equation 9
\begin{dmath}
log\left({{A}_{t}}\right)={{\rho^A}}\, log\left({{A}_{t-1}}\right)+{{\varepsilon^A}_{t}}
\end{dmath}
